q2

A1/test.dfy
@@ -1,29 +1,84 @@
-// Find minimum element in the array between left and right
+
+predicate sorted(a:array<int>, min:int, max:int)
+requires a != null;
+requires 0 <= min <= max < a.Length;
+reads a;
+{
+    forall j, k :: min <= j < k < max ==> a[j] <= a[k]
+}
+
+// Find maximum element in the array between left and right
 function method findMax (a: array<int>, left: int, right: int): int
     reads a;
     decreases right - left;
     requires a != null && a.Length > 0;
     requires 0 <= left <= right < a.Length;
     ensures  0 <= left <= right < a.Length;
-    ensures 0 <= findMax(a, left, right) < a.Length;
+    ensures  left <= findMax(a, left, right) <= right;
+    ensures forall i :: left <= i <= right ==> a[i] <= a[findMax(a, left, right)];
 {
     if (left < right) then 
         if (a[left] < a[right]) then 
             findMax(a, left + 1, right) 
         else findMax(a, left, right - 1) 
-    else 0
+    else right
 }
 
-method random(a: array <int>, left: int, right: int) 
+// Find minimum element in the array between left and right
+function method findMin (a: array<int>, left: int, right: int): int
+    reads a;
     decreases right - left;
     requires a != null && a.Length > 0;
     requires 0 <= left <= right < a.Length;
-    requires 0 <= findMax(a, left, right) < a.Length;
-    ensures 0 <= left <= right < a.Length;
+    ensures  0 <= left <= right < a.Length;
+    ensures  left <= findMin(a, left, right) <= right;
+    ensures forall i :: left <= i <= right ==> a[i] >= a[findMin(a, left, right)];
 {
+    if (left < right) then 
+        if (a[left] < a[right]) then 
+            findMin(a, left, right - 1) 
+        else findMin(a, left + 1, right) 
+    else left
+}
+
+method stoogeSort(a: array<int>, left: int, right: int)
+    modifies a;
+    requires a != null;
+    requires a.Length > 0;
+    requires 0 <= left <= right < a.Length;
+    requires 0 <= findMin(a, left, right) < a.Length;
+    requires 0 <= findMax(a, left, right) < a.Length;
+    
+    //ensures sorted(a, left, right);
+    /*
+        Making sure that whenever spawing happens
+        Only because it found an element that is smaller/bigger than previous ones
+    -*/
+    ensures a[left] <= old(a[left]);
+    ensures a[left] <= old(a[right]);
+    ensures a[right] >= old(a[right]);
+    ensures a[right] >= old(a[left]);
+    ensures a[left] <= a[right];
+
+    ensures a[left] == a[findMin(a, left, right)];
+    ensures a[right] == a[findMax(a, left, right)];
+    // ensures findMin(a, left, right) == old(findMin(a, left, right));
+    // ensures findMax(a, left, right) == old(findMax(a, left, right));
+    ensures forall i :: (0 <= i < left || right < i < a.Length) ==> a[i] == old(a[i]);
+    decreases right - left;
+{
+    if (a[left] > a[right])
+    {
+        // swap a[left] and a[right]
+        var tmp := a[left];
+        a[left] := a[right];
+        a[right] := tmp;
+    }
+	
     if (left + 1 >= right) {
         return;
-    }
-    random(a, left, right - 1); 
-    random(a, left + 1, right);
+	}
+    stoogeSort(a, left, right - 1);
+    stoogeSort(a, left + 1, right);
+    stoogeSort(a, left, right - 1);
 }
